Strata/Transform/CoreSpecification.lean
@@ -39,7 +39,8 @@ open Core Imperative
   Imperative.Specification.Lang.imperative
     Expression Command (EvalCommand π φ) (EvalPureFunc φ) coreIsAtAssert
     (fun s ρ => (∀ n ∈ Stmt.touchedVars s, (ρ.store n).isSome) ∧
-                WellFormedCoreEvalCong ρ.eval)
+                WellFormedCoreEvalCong ρ.eval ∧
+                WellFormedSemanticEvalExprCongr ρ.eval)
 
 /-! ## Well-formed program state at the entry of procedure -/
 
